io/ho_examples/Callback.Example.fst
@@ -4,16 +4,15 @@ open FStar.Tactics
 
 open Common
 open DM 
-open TC.ML
-open TC.ML.HO
+open ILang
+open IIO.Compile.Export
 open TC.Checkable
-open TC.Export
-open TC.MLify.IIOwp
-open TC.Monitorable.Hist
-open TC.Instrumentable.IIOwp
-  
-(** ** Callback example **)
+
 (** ***  accepts a function that accepts a callback **)
+(** pp  - partial program (TRUSTED)
+    ctx - context         (UNTRUSTED)
+    pp_cb - callback of partial program (TRUSTED) **)
+
 val pi : monitorable_prop
 let pi cmd arg h =
   match cmd with
@@ -21,33 +20,82 @@ let pi cmd arg h =
     let fnm : io_args Openfile = arg in not (fnm = "/tmp/passwd")
   | _ -> true
 
-unfold
-type cb  = fd:file_descr -> IIO (maybe bool) (fun h -> is_open fd h) (fun h _ lt -> lt == [])
-type ctx = cb:cb         -> IIO (maybe unit) (fun _ -> True)           (fun h r lt -> enforced_locally pi h lt)
-type pp  = f: ctx        -> IIO (maybe unit) (fun _ -> True)           (fun h r lt -> enforced_locally pi h lt)
+(** The type of the callback function.
+    The callback function in this example has non-higher-order types as input and output.
+    The callback is TRUSTED and it is passed by the main function to the UNTRUSTED side.
+    Thus, callback must be mlified before being past to the UNTRUSTED side.
+    Because the callback function is mlified, it means that the runtime checks can fail.
+    Because the UNTRUSTED side is instrumented to respect pi --- meaning that the post-conditon
+    of the UNTRUSTED side guarantees pi is respected --- the callback has also to respect pi.
+    Therefore, the callback function can be mlified only if it is part of the class mlifyable_in.
+**)
+unfold let pp_cb_in = file_descr
+val pp_cb_in_importable : importable pp_cb_in pi
+let pp_cb_in_importable = 
+  safe_importable_is_importable 
+    pp_cb_in 
+    #(ilang_is_safely_importable (ilang_file_descr pi))
+unfold let pp_cb_out = bool
+val pp_cb_out_exportable : exportable pp_cb_out pi
+let pp_cb_out_exportable = ilang_is_exportable pp_cb_out #(ilang_bool pi)
+val pp_cb_pre : pp_cb_in -> trace -> Type0
+let pp_cb_pre = fun fd h -> is_open fd h
+val pp_cb_post : pp_cb_in -> trace -> resexn pp_cb_out -> trace -> Type0
+let pp_cb_post = fun fd h _ lt -> lt == []
+type pp_cb = x:pp_cb_in -> IIO (resexn pp_cb_out) (pp_cb_pre x) (pp_cb_post x) 
 
-let cb_monitorable_hist : monitorable_hist (fun fd h -> is_open fd h) (fun fd h (x:maybe bool) lt -> lt == []) pi = {
+(** The UNTRUSTED side accepts the callback.
+    The UNTRUSTED side expects a callback that can fail.
+    Its pre-condition is a promise, thus is not verified dynamically.
+    Since the UNTRUSTED side is instrumented and its post-condition is dynamically
+    enforced, its output type must reflect the possibility of a contract failure.
+**)
+unfold let ctx_out = unit
+val ctx_out_importable : importable ctx_out pi
+let ctx_out_importable = 
+  safe_importable_is_importable 
+    ctx_out 
+    #(ilang_is_safely_importable (ilang_unit pi))
+val ctx_pre : pp_cb -> trace -> Type0
+let ctx_pre = fun _ _ -> true
+val ctx_post : pp_cb -> trace -> resexn ctx_out -> trace -> Type0
+let ctx_post = fun _ h _ lt -> enforced_locally pi h lt
+type ctx = x:pp_cb -> IIO (resexn ctx_out) (ctx_pre x) (ctx_post x)
+
+unfold let pp_out = unit
+val pp_out_exportable : exportable pp_out pi
+let pp_out_exportable = ilang_is_exportable pp_out #(ilang_unit pi)
+val pp_pre : ctx -> trace -> Type0
+let pp_pre = fun _ _ -> true
+val pp_post : ctx -> trace -> resexn pp_out -> trace -> Type0
+let pp_post = fun _ h _ lt -> enforced_locally pi h lt
+type pp = x:ctx -> IIO (resexn pp_out) (pp_pre x) (pp_post x)
+
+val pp_cb_pre_checkable : checkable2 pp_cb_pre
+let pp_cb_pre_checkable = general_is_checkable2 file_descr trace (fun fd h -> is_open fd h)
+
+val pp_cb_monitorable_hist : monitorable_hist pp_cb_pre pp_cb_post pi
+let pp_cb_monitorable_hist = {
   c1post = admit ()
 }
 
-let cb_mlifyable : mlifyable cb pi = 
-  mlifyable_iiowp_trivialize_weaken_post
-    file_descr
-    bool
-    (fun fd h -> is_open fd h)
-    (fun fd h _ lt -> lt == [])
-    pi
-    #cb_monitorable_hist
-    
+let pp_cb_exportable : exportable pp_cb pi =
+  exportable_arrow_with_pre_post
+    pp_cb_in #pp_cb_in_importable
+    pp_cb_out #pp_cb_out_exportable
+    pp_cb_pre #pp_cb_pre_checkable
+    pp_cb_post
+    #pp_cb_monitorable_hist
 
 private
-let lemma_c1post () : squash (forall (x:cb_mlifyable.matype) h lt. True /\ enforced_locally pi h lt ==> (exists (r:maybe unit). enforced_locally pi h lt)) by (explode (); witness (`(Inl ())))= ()
+let lemma_c1post () : squash (forall (x:pp_cb) h lt. true /\ enforced_locally pi h lt ==> (exists (r:resexn unit). enforced_locally pi h lt)) by (explode (); witness (`(Inl ())))= ()
 
 private
 let lemma_c2post () : squash (forall h lt. enforced_locally pi h lt  ==> enforced_locally pi h lt) =
   lemma_c1post ()
 
-let pp_post_monitorable : checkable_hist_post (fun fd h -> True) (fun fd h r lt -> enforced_locally pi h lt) pi = {
+val ctx_checkable_hist : checkable_hist_post #pp_cb ctx_pre ctx_post pi
+let ctx_checkable_hist = {
   cmonitorable = {
     c1post = lemma_c1post ();
   };
@@ -55,33 +103,47 @@ let pp_post_monitorable : checkable_hist_post (fun fd h -> True) (fun fd h r lt 
   c2post = lemma_c2post ();
 }
 
-unfold
-let ctx_instrumentable : instrumentable ctx pi =
-  instrumentable_HO_arr1_out_importable
-    cb
-    unit (fun h -> True) (fun h r lt -> enforced_locally pi h lt) 
-    pi
-    #(importable_safe_importable _ #(safe_importable_ml (maybe unit) #(mlfo_maybe unit #(ML_FO mlfo_unit))))
-    #cb_mlifyable
-    #pp_post_monitorable
+let ctx_importable : importable ctx pi =
+  safe_importable_is_importable ctx #(
+    safe_importable_arrow_pre_post
+      pp_cb #pp_cb_exportable
+      ctx_out #ctx_out_importable
+      ctx_pre
+      ctx_post
+      #ctx_checkable_hist)
+
+val pp_pre_checkable : checkable2 pp_pre
+let pp_pre_checkable = general_is_checkable2 ctx trace (fun _ _ -> true)
   
-let pp_mlifyable : mlifyable pp (trivial_pi ()) =
-  mlifyable_inst_iiowp_weaken ctx #ctx_instrumentable (maybe unit) (fun h r lt -> enforced_locally pi h lt)
+val pp_monitorable_hist : monitorable_hist pp_pre pp_post pi
+let pp_monitorable_hist = {
+  c1post = admit ()
+}
 
-let main : pp = fun c ->
-  let theCb : cb = fun fd -> if is_open fd (get_trace ()) then Inl true else Inl false in
-  c theCb
+let pp_exportable: exportable pp pi =
+  exportable_arrow_with_pre_post
+    ctx #ctx_importable
+    pp_out #pp_out_exportable
+    pp_pre #pp_pre_checkable
+    pp_post
+    #pp_monitorable_hist
 
-val c : ctx_instrumentable.inst_type
-//let c (theCb : file_descr -> IIOpi (maybe bool) pi) : IIOpi (maybe unit) pi =
-let c (theCb : cb_mlifyable.matype) : IIOpi (maybe unit) pi =
+let thePP : pp = fun theCtx ->
+  let theCb : pp_cb = fun fd -> if is_open fd (get_trace ()) then Inl true else Inl false in
+  theCtx theCb
+
+exception Error_just_for_example
+
+val theCtx : ctx_importable.itype
+//let theCtx (theCb : file_descr -> IIOpi (resexn bool) pi) : IIOpi (resexn unit) pi =
+let theCtx (theCb : pp_cb_exportable.etype) : IIOpi (resexn unit) pi =
   let fd = static_cmd Openfile "/tmp2/passwd" in
   if Inl? fd  then
     let test = theCb (Inl?.v fd) in
     if Inl? test && Inl?.v test then Inl ()
-    else Inr Something_went_really_bad
-  else Inr Something_went_really_bad
+    else Inr Error_just_for_example
+  else Inr Error_just_for_example
 
-let main_mlify = mlify #_ #_ #pp_mlifyable main
+let main_mlify = export #_ #_ #pp_exportable thePP
 
-let whole () : MIIO (maybe unit) = main_mlify c
+let whole () : IIOpi (resexn unit) pi = main_mlify theCtx
